type inference is sound!

ML_SP_Inference.v
@@ -16,6 +16,36 @@ Section Index.
     | nil   => None
     | y::l' => if eq_dec x y then Some i else index (S i) x l'
     end.
+
+  Lemma index_none_notin : forall x l n,
+    index n x l = None -> ~In x l.
+  Proof.
+    induction l; simpl; intros. auto.
+    destruct* (eq_dec x a). discriminate.
+  Qed.
+
+  Lemma index_ok : forall (B:Set) (f:A->B) (def:B) a l n,
+    index 0 a l = Some n ->
+    nth n (List.map f l) def = f a.
+  Proof.
+    intros.
+    replace n with (n-0) by omega.
+    apply (proj2 (A:= 0 <= n)).
+    gen n; generalize 0.
+    induction l; simpl; intros. discriminate.
+    destruct (eq_dec a a0).
+      subst.
+      inversions H.
+      split*.
+      replace (n0 - n0) with 0 by omega.
+      auto.
+    destruct (IHl _ _ H).
+    split. omega.
+    case_eq (n0 - n); intros.
+      elimtype False; omega.
+    replace n2 with (n0 - S n) by omega.
+    auto.
+  Qed.
 End Index.
 
 Require Import ML_SP_Definitions ML_SP_Infrastructure.
@@ -45,9 +75,28 @@ Definition unify K T1 T2 S :=
 Definition fvs S K E T :=
   dom S \u fv_in typ_fv S \u dom K \u fv_in kind_fv K \u env_fv E \u typ_fv T.
 
+(** Variants looking up a kinding environment *)
+
+Fixpoint close_fvars (n:nat)(K:kenv)(VK:vars)(Vs:vars) {struct n} : vars :=
+  match n with
+  | 0 => Vs
+  | S n' =>
+    match S.choose (S.inter VK Vs) with
+    | None => Vs
+    | Some x =>
+      let VK' := S.remove x VK in
+      let Vs' :=
+        match get x K with
+        | None => Vs
+        | Some k => Vs \u kind_fv k
+        end
+      in close_fvars n' K VK' Vs'
+    end
+  end.
+    
 Definition close_fvk K := close_fvars (length K) K (dom K).
 
-Fixpoint generalize (Bs:list var) (T:typ) {struct T} : typ :=
+Fixpoint typ_generalize (Bs:list var) (T:typ) {struct T} : typ :=
   match T with
   | typ_bvar n =>
     typ_bvar (length Bs + n)
@@ -57,8 +106,11 @@ Fixpoint generalize (Bs:list var) (T:typ) {struct T} : typ :=
     | Some n => typ_bvar n
     end
   | typ_arrow T1 T2 =>
-    typ_arrow (generalize Bs T1) (generalize Bs T2)
+    typ_arrow (typ_generalize Bs T1) (typ_generalize Bs T2)
   end.
+
+Definition sch_generalize Bs T Ks :=
+  Sch (typ_generalize Bs T) (List.map (kind_map (typ_generalize Bs)) Ks).
 
 Fixpoint split_env (A:Set) (B:vars) (E:env A) {struct E} : env A * env A :=
   match E with
@@ -102,14 +154,13 @@ Fixpoint typinf (K:kenv) (E:Defs.env) (t:trm) (T:typ) (S:subs) (h:nat)
       let K' := Env.map (kind_subst S') K0 in
       let E' := Env.map (sch_subst S') E in
       let ftve := close_fvk K' (env_fv E' \u vars_subst S' (dom K)) in
+      let (K'', KA) := split_env ftve K' in
       let T1 := typ_subst S' V in
-      let B := S.diff (close_fvk K' (typ_fv T1)) ftve in
-      let (Kb, KB) := split_env B K' in
+      let B := close_fvk K' (typ_fv T1) in
+      let (_, KB) := split_env B K'' in
       let (Bs, Ks) := split KB in
       let x := proj1_sig (var_fresh (dom E \u trm_fv t1 \u trm_fv t2)) in
-      typinf Kb
-        (E & x~Sch (generalize Bs T1) (List.map (kind_map (generalize Bs)) Ks))
-        (t2 ^ x) T S' h'
+      typinf KA (E & x ~ sch_generalize Bs T1 Ks) (t2 ^ x) T S' h'
     end
   | trm_app t1 t2 =>
     let V := typ_fvar (proj1_sig (var_fresh (fvs S K E T))) in
@@ -312,8 +363,8 @@ Proof.
 Qed.
 Lemma split_env_ok : forall (A:Set) (B:vars) (E Eb EB:env A),
   split_env B E = (Eb, EB) -> ok E ->
-  ok (Eb & EB) /\ disjoint B (dom Eb) /\ dom EB << B /\
-  env_incl E (Eb & EB) /\ env_incl (Eb & EB) E.
+  ok (EB & Eb) /\ disjoint B (dom Eb) /\ dom EB << B /\
+  env_incl E (EB & Eb) /\ env_incl (EB & Eb) E.
 Proof.
   induction E; simpl; intros.
     inversions H. simpl. split*. split. intro; auto*.
@@ -328,7 +379,7 @@ Proof.
     inversions H0; clear H0.
     destruct* (IHE Eb e0) as [Hok [Dis [Dom [I1 I2]]]]; clear IHE.
     destruct (ok_concat_inv _ _ Hok).
-    case_eq (get v (Eb & e0)); intros.
+    case_eq (get v (e0 & Eb)); intros.
       elim (binds_fresh (I2 _ _ H1) H4).
     poses Hv' (get_none_notin _ H1); clear H1.
     split.
@@ -346,11 +397,12 @@ Proof.
     replace ((v,a) :: E) with (E & v ~ a) by simpl*.
     replace ((v,a) :: e0) with (e0 & v ~ a) by simpl*.
     split; intro; intros; binds_cases H1; auto*.
+    use (I1 _ _ B0). binds_cases H1; auto*.
   inversions H; clear H.
   inversions H0; clear H0.
   destruct* (IHE e EB) as [Hok [Dis [Dom [I1 I2]]]]; clear IHE.
   destruct (ok_concat_inv _ _ Hok).
-  case_eq (get v (e & EB)); intros.
+  case_eq (get v (EB & e)); intros.
     elim (binds_fresh (I2 _ _ H1) H4).
   poses Hv' (get_none_notin _ H1); clear H1.
   split.
@@ -366,8 +418,6 @@ Proof.
   replace ((v,a) :: E) with (E & v ~ a) by simpl*.
   replace ((v,a) :: e) with (e & v ~ a) by simpl*.
   split; intro; intros; binds_cases H1; auto*.
-  use (I1 _ _ B0).
-  binds_cases H1; auto*.
 Qed.
 
 Lemma proper_instance_well_subst : forall S K K' M Us,
@@ -622,7 +672,7 @@ Proof.
   apply* kind_subst_entails.
 Qed.
 
-Definition soundness_spec h t K0 E T S0 K S gc :=
+Definition soundness_spec h t K0 E T S0 K S :=
   typinf K0 E t T S0 h = Some (K, S) ->
   is_subst S0 -> env_prop type S0 ->
   kenv_ok K0 -> disjoint (dom S0) (dom K0) ->
@@ -630,18 +680,24 @@ Definition soundness_spec h t K0 E T S0 K S gc :=
   extends S S0 /\ env_prop type S /\ is_subst S /\
   kenv_ok K /\ disjoint (dom S) (dom K) /\
   well_subst (map (kind_subst S0) K0) (map (kind_subst S) K) S /\
-  map (kind_subst S) K; map (sch_subst S) E | gc |= t ~: typ_subst S T.
+  map (kind_subst S) K; map (sch_subst S) E |(true,GcAny)|= t ~: typ_subst S T.
           
-Lemma soundness_var : forall h v K0 E T S0 K S gc,
-  soundness_spec (Datatypes.S h) (trm_fvar v) K0 E T S0 K S gc.
+Lemma soundness_ind : forall h t K0 E T S0 K S s x,
+  scheme s ->
+  fresh (fvs S0 K0 E T) (sch_arity s) x ->
+  unify (K0 & kinds_open_vars (sch_kinds s) x) (sch_open_vars s x) T S0 =
+    Some (K, S) ->
+  (kenv_ok (K0 & kinds_open_vars (sch_kinds s) x) ->
+   extends S S0 -> kenv_ok K ->
+   unifies S ((sch_open_vars s x, T) :: nil) ->
+   map (kind_subst S0) (K0 & kinds_open_vars (sch_kinds s) x);
+   map (sch_subst S0) E |(true, GcAny)|= t ~: sch_subst S0 s ^^ typ_fvars x) ->
+  soundness_spec h t K0 E T S0 K S.
 Proof.
-  intros until gc; intros HI HS0 HTS0 HK0 Dis HE HSE HT; simpl in HI.
-  case_rewrite (get v E) R1.
-  destruct (var_freshes (fvs S0 K0 E T) (sch_arity s)).
-  simpl proj1_sig in HI.
+  intros until x; intros Hs f HI Typ _ HS0 HTS0 HK0 Dis HE HSE HT.
   unfold unify in HI.
   assert (kenv_ok (K0 & kinds_open_vars (sch_kinds s) x)).
-    apply* kenv_ok_sch_kinds. apply* (HSE v).
+    apply* kenv_ok_sch_kinds.
     unfold fvs in f; auto.
   destruct* (unify_kinds_ok _ _ HI HS0).
     unfold fvs in f. rewrite dom_concat. rewrite* dom_kinds_open_vars.
@@ -653,7 +709,7 @@ Proof.
     inversions H2; clear H2.
     split*.
     unfold sch_open_vars.
-    refine (proj1 (HSE _ _ R1 x _)). auto.
+    destruct* (Hs x).
   intuition.
       destruct* (unify_keep _ _ _ HI).
     intro; intros.
@@ -664,31 +720,95 @@ Proof.
     apply* ok_map0.
   rewrite <- (map_sch_subst_extend E Hext).
   use (unify_types _ _ _ HI HS0).
-  rewrite* <- (H1 (sch_open_vars s x) T).
-  rewrite* <- (typ_subst_extend _ _ _ HS0 HI).
+  rewrite* <- (H6 (sch_open_vars s x) T).
+  rewrite* <- Hext.
   unfold fvs in f.
   rewrite* sch_subst_open_vars.
   apply* typing_typ_well_subst.
-    apply* kenv_ok_map.
-  unfold sch_open_vars, typ_open_vars.
-  fold (sch_open (sch_subst S0 s) (typ_fvars x)).
+  apply* kenv_ok_map.
+Qed.
+
+Lemma well_kinded_open_vars : forall S K Ks Xs,
+  fresh (dom S \u dom K) (length Ks) Xs ->
+  env_prop type S ->
+  For_all2
+     (well_kinded (map (kind_subst S) (K & kinds_open_vars Ks Xs)))
+     (kinds_open (List.map (kind_subst S) Ks) (typ_fvars Xs))
+     (typ_fvars Xs).
+Proof.
+  unfold kinds_open_vars, kinds_open; intros.
+  rewrite map_concat.
+  rewrite map_combine.
+  rewrite map_map.
+  rewrite <- (map_ext (fun k => kind_open (kind_subst S k) (typ_fvars Xs))).
+    rewrite <- (map_map (kind_subst S) (fun k => kind_open k (typ_fvars Xs))).
+    refine (well_kinded_combine _ _ Xs nil _).
+    rewrite dom_map.
+    rewrite* map_length.
+  intros. rewrite* kind_subst_open_vars.
+Qed.
+
+Lemma soundness_var : forall h v K0 E T S0 K S,
+  soundness_spec (Datatypes.S h) (trm_fvar v) K0 E T S0 K S.
+Proof.
+  intros; intros HI HS0 HTS0 HK0 Dis HE HSE HT.
+  poses HI' HI; simpl in HI.
+  case_rewrite (get v E) R1.
+  destruct (var_freshes (fvs S0 K0 E T) (sch_arity s)).
+  unfold fvs in f.
+  simpl proj1_sig in HI.
+  refine (soundness_ind _ _ _ _ HI _ HI' _ _ _ _ _ _ _); auto.
+    apply (HSE _ _ R1).
+  intros.
   apply* typing_var.
     apply* kenv_ok_map.
   split.
     unfold sch_arity. simpl. rewrite map_length. fold (sch_arity s).
     rewrite (fresh_length _ _ _ f). apply types_typ_fvars.
   split. apply* sch_subst_type. apply (HSE _ _ R1).
-  unfold kinds_open_vars, kinds_open.
-  rewrite map_concat.
-  rewrite map_combine.
-  rewrite map_map.
-  rewrite <- (map_ext (fun k => kind_open (kind_subst S0 k) (typ_fvars x))).
-    rewrite <- (map_map (kind_subst S0) (fun k => kind_open k (typ_fvars x))).
-    destruct s as [Ts Ks]; simpl.
-    refine (well_kinded_combine _ _ x nil _).
-    rewrite dom_map. rewrite map_length.
-    unfold sch_arity, fvs in f; simpl in f; auto.
-  intros. rewrite* kind_subst_open_vars.
+  destruct s as [Ts Ks]; simpl.
+  apply* well_kinded_open_vars.
+Qed.
+
+Lemma kinds_subst_cst : forall S c,
+  List.map (kind_subst S) (sch_kinds (Delta.type c)) = sch_kinds (Delta.type c).
+Proof.
+  intros.
+  assert (forall x, x \notin kind_fv_list (sch_kinds (Delta.type c))).
+    intros x Hx.
+    assert (x \in sch_fv (Delta.type c)).
+      unfold sch_fv.
+      auto with sets.
+    rewrite Delta.closed in H.
+    elim (in_empty H).
+  induction (sch_kinds (Delta.type c)). auto.
+  simpl in *.
+  rewrite* IHl.
+    rewrite* kind_subst_fresh.
+    intro. use (H x).
+  intro; use (H x).
+Qed.
+
+Lemma soundness_cst : forall h c K0 E T S0 K S,
+  soundness_spec (Datatypes.S h) (trm_cst c) K0 E T S0 K S.
+Proof.
+  intros; intros HI HS0 HTS0 HK0 Dis HE HSE HT.
+  poses HI' HI; simpl in HI.
+  destruct (var_freshes (fvs S0 K0 E T) (sch_arity (Delta.type c)));
+    simpl in HI.
+  refine (soundness_ind _ _ _ _ HI _ HI' _ _ _ _ _ _ _); auto.
+    apply Delta.scheme.
+  intros.
+  rewrite sch_subst_fresh; try (rewrite Delta.closed; intro; auto).
+  apply* typing_cst.
+    apply* kenv_ok_map.
+  split.
+    rewrite (fresh_length _ _ _ f). apply types_typ_fvars.
+  split. apply Delta.scheme.
+  pattern (sch_kinds (Delta.type c)) at 2.
+  rewrite <- (kinds_subst_cst S0 c).
+  unfold fvs, sch_arity in f.
+  apply* well_kinded_open_vars.
 Qed.
 
 Lemma typing_abs_rename : forall x1 gc K E x2 M t T,
@@ -717,11 +837,11 @@ Proof.
   rewrite* H0.
 Qed.
 
-Lemma soundness_abs : forall h t K0 E T S0 K S gc,
-  (forall t K0 E T S0 K S gc, soundness_spec h t K0 E T S0 K S gc) ->
-  soundness_spec (Datatypes.S h) (trm_abs t) K0 E T S0 K S gc.
+Lemma soundness_abs : forall h t K0 E T S0 S K,
+  (forall t K0 E T S0 K S, soundness_spec h t K0 E T S0 K S) ->
+  soundness_spec (Datatypes.S h) (trm_abs t) K0 E T S0 K S.
 Proof.
-  intros until gc; intros IHh  HI HS0 HTS0 HK0 Dis HE HSE HT; simpl in HI.
+  intros until K; intros IHh  HI HS0 HTS0 HK0 Dis HE HSE HT; simpl in HI.
   destruct (var_fresh (fvs S0 K0 E T)); simpl in HI.
   destruct (var_fresh (fvs S0 K0 E T \u {{x}})); simpl in HI.
   destruct (var_fresh (dom E \u trm_fv t)); simpl in HI.
@@ -733,7 +853,7 @@ Proof.
     simpl; intros. destruct* H.
     inversions* H.
   destruct* (unify_kinds_ok _ _ R1). clear H1; destruct H2.
-  destruct* (IHh _ _ _ _ _ _ _ gc HI); clear IHh HI.
+  destruct* (IHh _ _ _ _ _ _ _ HI); clear IHh HI.
       apply* ok_cons.
     intro; intros.
     assert (binds x2 a (E & x1 ~ Sch (typ_fvar x) nil)) by apply H3.
@@ -754,7 +874,7 @@ Proof.
   fold (typ_subst S (typ_fvar x0)).
   fold (typ_subst S (typ_fvar x)).
   set (E' := map (sch_subst S) E) in *.
-  apply* (@typing_abs gc (dom E' \u {{x1}} \u trm_fv t)).
+  apply* (@typing_abs (true,GcAny) (dom E' \u {{x1}} \u trm_fv t)).
   intros.
   apply typing_gc_raise.
   apply* (@typing_abs_rename x1).
@@ -770,128 +890,165 @@ Proof.
   use (get_none_notin _ H0).
 Qed.
 
+Lemma typ_generalize_reopen : forall Xs T,
+  type T -> typ_open (typ_generalize Xs T) (typ_fvars Xs) = T.
+Proof.
+  induction 1; simpl.
+    case_eq (index eq_var_dec 0 X Xs); simpl; intros.
+      unfold typ_fvars.
+      apply* index_ok.
+    auto.
+  congruence.
+Qed.
+
+Lemma kind_generalize_reopen : forall Xs k,
+  All_kind_types type k ->
+  kind_open (kind_map (typ_generalize Xs) k) (typ_fvars Xs) = k.
+Proof.
+  unfold All_kind_types.
+  intros; destruct k as [[kc kv kr kh]|]; simpl in *; auto.
+  apply kind_pi; simpl*.
+  clear kh; induction kr; simpl*.
+  destruct a. simpl in *.
+  rewrite* typ_generalize_reopen. rewrite* IHkr.
+Qed.
+
+Lemma kinds_generalize_reopen : forall Xs Ks,
+  list_forall (All_kind_types type) Ks ->
+  kinds_open_vars (List.map (kind_map (typ_generalize Xs)) Ks) Xs =
+  combine Xs Ks.
+Proof.
+  unfold kinds_open_vars, kinds_open; intros.
+  apply (f_equal (combine (B:=kind) Xs)).
+  induction H; simpl. auto.
+  rewrite* kind_generalize_reopen.
+  congruence.
+Qed.
+
 Lemma type_generalize : forall Bs Xs T,
   length Bs = length Xs ->
   type T ->
-  type (typ_open_vars (generalize Bs T) Xs).
+  type (typ_open_vars (typ_generalize Bs T) Xs).
 Proof.
   intros.
-  unfold typ_open_vars, typ_fvars.
-  induction H0; simpl.
-    set (n := 0).
-    assert (n + length Bs = length Xs) by auto.
-    clear H; clearbody n.
-    gen n; induction Bs; simpl; intros. auto.
-    destruct (X == a). subst.
-      simpl.
-      clear IHBs.
-      gen Xs; induction n; destruct Xs; simpl; intros; try discriminate; auto.
-    apply IHBs. omega.
-  auto.
+  apply* (typ_open_vars_type Bs).
+  unfold typ_open_vars.
+  rewrite* typ_generalize_reopen.
 Qed.
 
 Lemma scheme_generalize : forall Bs Ks T,
   length Bs = length Ks ->
   type T -> list_forall (All_kind_types type) Ks ->
-  scheme (Sch (generalize Bs T) (List.map (kind_map (generalize Bs)) Ks)).
+  scheme (sch_generalize Bs T Ks).
 Proof.
   intros.
   intro; simpl; intros.
   rewrite map_length in H2.
   rewrite H2 in H.
   split. apply* type_generalize.
-  set (Ks' := Ks). fold Ks' in H1.
-  clearbody Ks'.
-  induction H1; simpl. auto.
-  constructor; auto.
+  apply* list_forall_map; intros.
   apply All_kind_types_map.
   apply* All_kind_types_imp; intros.
   apply* type_generalize.
 Qed.
 
-Lemma close_fvk_incl : forall L K,
-  L << close_fvk K L.
+Lemma close_fvars_subset : forall K n DK L,
+  L << close_fvars n K DK L.
 Proof.
-  intros L K x Hx.
-  unfold close_fvk.
-  gen L. generalize (dom K).
-  induction (length K); simpl; intros. auto.
-  case_eq (S.choose (S.inter v L)); introv R1; auto.
-  case_eq (get e K); introv R2; auto.
-  apply* IHn. auto with sets.
+  induction n; intros; simpl; intros x Hx. auto.
+  case_eq (S.choose (S.inter DK L)); introv R1; auto.
+  case_eq (get e K); introv R2; apply* IHn; auto with sets.
 Qed.
 
-Lemma soundness_let : forall h t1 t2 K0 E T S0 K S gc,
-  (forall t K0 E T S0 K S gc, soundness_spec h t K0 E T S0 K S gc) ->
-  soundness_spec (Datatypes.S h) (trm_let t1 t2) K0 E T S0 K S gc.
+Lemma close_fvk_subset : forall L K, L << close_fvk K L.
 Proof.
-  intros until gc; intros IHh  HI HS0 HTS0 HK0 Dis HE HSE HT; simpl in HI.
-  destruct (var_fresh (fvs S0 K0 E T)); simpl in HI.
-  case_rewrite (typinf K0 E t1 (typ_fvar x) S0 h) R1. destruct p.
-  fold (typ_subst s (typ_fvar x)) in HI.
-  set (K' := map (kind_subst s) k) in *.
-  case_rewrite (split_env
-             (S.diff (close_fvk K' (typ_fv (typ_subst s (typ_fvar x))))
-               (close_fvk K'
-                 (env_fv (map (sch_subst s) E) \u vars_subst s (dom K0))))
-           K') R2.
-  case_rewrite (split e0) R3.
-  destruct (var_fresh (dom E \u trm_fv t1 \u trm_fv t2)); simpl proj1_sig in HI.
-  destruct* (IHh _ _ _ _ _ _ _ gc R1); clear R1.
-  destruct H0 as [HTs [Hs [Hk [Disk [WS' Typ']]]]].
-  assert (HK':kenv_ok K'). unfold K'; apply* kenv_ok_map.
-  destruct* (split_env_ok _ R2) as [Ok [Dise [Se0 [Inc1 Inc2]]]].
-  destruct* (IHh _ _ _ _ _ _ _ gc HI); clear IHh HI.
-          split. destruct* (ok_concat_inv _ _ Ok).
-          intro; intros.
-          apply (proj2 HK' x1).
-          apply* (Inc2 x1).
-        use (env_incl_subset_dom Inc2).
-        unfold K' in H0; rewrite dom_map in H0; rewrite dom_concat in H0.
-        intro v; destruct* (Disk v).
-        use (notin_subset H0 H1).
-      apply* ok_cons.
-    intro; intros.
-    unfold binds in H0; simpl in H0.
-    destruct (x1 == x0); subst.
-      inversions H0; clear H0.
-      fold (typ_subst s (typ_fvar x)).
-      use (split_length_l e0).
-      rewrite <- (split_length_r e0) in H0.
-      rewrite R3 in H0; simpl in H0.
-      apply* scheme_generalize.
-      use (split_combine e0). rewrite R3 in H1.
-      apply* env_prop_list_forall.
-        rewrite H1.
-        intro; intros.
-        apply* (proj2 HK' x1).
-      rewrite H1.
-      destruct* (ok_concat_inv _ _ Ok).
-    apply (HSE _ _ H0).
-  intuition.
-      apply* extends_trans.
-    intro; intros.
-    use (WS' _ _ H6).
-    inversions H8.
-      destruct k0; try discriminate; apply wk_any.
-    fold (typ_subst s (typ_fvar Z)) in H10.
-    rewrite* <- (kind_subst_combine S S s). rewrite <- H9.
-    rewrite <- H0. rewrite <- H10.
-    rewrite <- H9 in H8; rewrite <- H10 in H8.
-    rewrite <- (map_compose (kind_subst s) (kind_subst s) (kind_subst s))
-      in H12.
-    destruct (binds_map_inv _ _ H12) as [k2 [Hk2 B]].
-    use (Inc1 _ _ B).
-    binds_cases H11.
-      use (binds_map (kind_subst s) B0).
-      use (H5 _ _ H11).
-      rewrite Hk2 in H14.
-      apply* kind_entails_well_kinded.
-      simpl; apply* kind_subst_entails.
-    use (S.diff_2 (Se0 _ (binds_dom B1))).
-    use (notin_subset (close_fvk_incl _) H11).
-    use (binds_dom H6).
-    rewrite dom_map in H15.
+  intros. unfold close_fvk. apply close_fvars_subset.
+Qed.
+
+Hint Resolve close_fvk_subset.
+
+Require Import Cardinal.
+
+Lemma cardinal_empty : S.cardinal {} = 0.
+Proof.
+  rewrite S.cardinal_1.
+  case_eq (S.elements {}); intros. simpl*.
+  assert (In e (e::l)) by auto.
+  rewrite <- H in H0.
+  assert (e \in {}). auto with sets.
+  elim (in_empty H1).
+Qed.
+
+Lemma cardinal_env : forall (A:Set) (K:env A),
+  ok K -> S.cardinal (dom K) = length K.
+Proof.
+  induction 1; simpl. apply cardinal_empty.
+  rewrite <- (@cardinal_remove x).
+    rewrite remove_union.
+    assert (S.remove x {{x}} = {}).
+      apply eq_ext; intros; split; intros.
+        use (S.remove_3 H1).
+        elim (S.remove_1 (S.singleton_1 H2) H1).
+      elim (in_empty H1).
+    rewrite H1. rewrite* remove_notin.
+    rewrite* union_empty_l.
+  auto with sets.
+Qed.
+
+Lemma cardinal_0 : forall L,
+  S.cardinal L = 0 -> L = {}.
+Proof.
+  intros.
+  rewrite S.cardinal_1 in H.
+  case_rewrite (S.elements L) R1.
+  apply eq_ext; intros; split; intro; intros.
+    use (S.elements_1 H0).
+    rewrite R1 in H1.
+    inversion H1.
+  elim (in_empty H0).
+Qed.
+
+Lemma close_fvk_ok : forall K L x k,
+  ok K -> x \in close_fvk K L -> binds x k K -> kind_fv k << close_fvk K L.
+Proof.
+  intros.
+  unfold close_fvk in *.
+  use (cardinal_env H).
+  use (binds_dom H1).
+  revert L H0 H2 H3; generalize (dom K).
+  induction (length K); simpl; intros.
+    rewrite (cardinal_0 H2) in *. elim (in_empty H3).
+  case_rewrite (S.choose (S.inter v L)) R1.
+    use (S.choose_1 R1).
+    destruct (x == e).
+      subst.
+      rewrite H1 in *.
+      intros x Hx.
+      apply close_fvars_subset. auto with sets.
+    assert (forall L', x \in close_fvars n K (S.remove e v) L' ->
+               kind_fv k << close_fvars n K (S.remove e v) L').
+      intros; apply* IHn.
+        rewrite <- (@cardinal_remove e) in H2; auto.
+        eauto with sets.
+      apply* S.remove_2.
+    case_rewrite (get e K) R2; intros; auto.
+  use (S.choose_2 R1).
+  elim (H4 x).
+  auto with sets.
+Qed.
+
+
+Lemma split_length : forall (A B:Set) l (l1:list A) (l2:list B),
+  split l = (l1, l2) -> length l1 = length l2.
+Proof.
+  intros.
+  use (split_length_l l).
+  rewrite <- (split_length_r l) in H0.
+  rewrite H in H0; apply H0.
+Qed.
+
+Hint Resolve split_length.
+
 Lemma vars_subst_in : forall v L S,
   v \in L -> typ_fv (typ_subst S (typ_fvar v)) << vars_subst S L.
 Proof.
@@ -903,24 +1060,436 @@ Proof.
   simpl.
   use (IHInA _ Hx). auto with sets.
 Qed.
-    elim H14.
-    apply S.union_3.
-    apply* (vars_subst_in s H15).
-    rewrite <- H10.
-    simpl. auto with sets.
-    intro; apply* kind_subst_idem.
-  set (M := Sch (generalize l (typ_subst s (typ_fvar x)))
-              (List.map (kind_map (generalize l)) l0)) in *.
-  apply* (@typing_let gc (sch_subst S M) (dom K)).
-    intros.
 
-Theorem soundness : forall h t K0 E T S0 K S gc,
-  soundness_spec h t K0 E T S0 K S gc.
+Lemma sch_arity_subst : forall M S,
+  sch_arity (sch_subst S M) = sch_arity M.
+Proof.
+  destruct M as [T Ks]; unfold sch_arity. simpl.
+  intro; rewrite* map_length.
+Qed.
+
+Hint Resolve kind_subst_idem.
+
+Lemma disjoint_subset : forall L1 L2 L3,
+  L1 << L2 -> disjoint L2 L3 -> disjoint L1 L3.
+Proof.
+  intros. disjoint_solve. auto.
+Qed.
+
+Lemma well_subst_let_inf : forall S0 K0 s k e e0 S K L,
+  extends S s -> is_subst s ->
+  well_subst (map (kind_subst S0) K0) (map (kind_subst s) k) s ->
+  well_subst (map (kind_subst s) e0) (map (kind_subst S) K) S ->
+  let K' := map (kind_subst s) k in
+  env_incl K' (e0 & e) ->
+  disjoint (close_fvk K' (L \u vars_subst s (dom K0))) (dom e) ->
+  well_subst (map (kind_subst S0) K0) (map (kind_subst S) K) S.
+Proof.
+  intros until L; intros Hext Hs WS WS' K' Inc1 Dise; intro; intros.
+  use (WS _ _ H).
+  inversions H0.
+    destruct k0; try discriminate; apply wk_any.
+  fold (typ_subst s (typ_fvar Z)) in H2.
+  rewrite* <- (kind_subst_combine S S s). rewrite <- H1.
+  rewrite <- Hext. rewrite <- H2.
+  rewrite <- H1 in H0; rewrite <- H2 in H0.
+  rewrite <- (map_compose (kind_subst s) (kind_subst s) (kind_subst s))
+    in H4; auto*.
+  destruct (binds_map_inv _ _ H4) as [k2 [Hk2 B]].
+  use (Inc1 _ _ B).
+  binds_cases H3.
+    use (binds_map (kind_subst s) B0).
+    use (WS' _ _ H3).
+    rewrite Hk2 in H6.
+    apply* kind_entails_well_kinded.
+    simpl; apply* kind_subst_entails.
+  use (binds_dom B1).
+  destruct* (Dise x).
+  use (notin_subset (close_fvk_subset _) H6).
+  use (binds_dom H).
+  rewrite dom_map in H8.
+  elim H7; clear H6 H7.
+  apply S.union_3.
+  apply* (vars_subst_in s H8).
+  rewrite <- H2.
+  simpl. auto with sets.
+Qed.
+
+Lemma in_ok_binds : forall (A:Set) x (a:A) E,
+  In (x,a) E -> ok E -> binds x a E.
+Proof.
+  intros.
+  unfold binds.
+  induction H0. elim H.
+  simpl.
+  simpl in H; destruct H.
+    inversions H.
+    destruct* (x == x).
+  destruct* (x == x0).
+  subst.
+  elim (binds_fresh (IHok H) H1).
+Qed.
+
+Lemma mkset_notin : forall x l, ~In x l -> x \notin mkset l.
+Proof.
+  induction l; simpl; intros. auto.
+  intuition.
+  destruct* (S.union_1 H0).
+  elim H1; rewrite* (S.singleton_1 H3).
+Qed.
+Hint Resolve mkset_notin.
+
+Lemma typ_generalize_disjoint : forall Bs T,
+  disjoint (typ_fv (typ_generalize Bs T)) (mkset Bs).
+Proof.
+  induction T; simpl. intro; auto.
+    case_eq (index eq_var_dec 0 v Bs); simpl; intros.
+      intro; auto.
+    use (index_none_notin _ _ _ _ H).
+  disjoint_solve.
+Qed.
+
+Lemma kinds_generalize_disjoint : forall Bs Ks,
+  disjoint (kind_fv_list (List.map (kind_map (typ_generalize Bs)) Ks))
+    (mkset Bs).
+Proof.
+  intros. unfold kind_fv_list.
+  induction Ks; simpl. intro; auto.
+  apply* disjoint_union.
+  unfold kind_fv.
+  clear IHKs Ks; destruct a as [[kc kv kr kh]|]; simpl.
+    clear kh; induction kr; simpl. intro; auto.
+    apply* disjoint_union.
+    apply typ_generalize_disjoint.
+  intro; auto.
+Qed.
+
+Lemma sch_generalize_disjoint : forall Bs T Ks,
+  disjoint (sch_fv (sch_generalize Bs T Ks)) (mkset Bs).
+Proof.
+  intros.
+  unfold sch_generalize, sch_fv; simpl.
+  apply disjoint_union. apply typ_generalize_disjoint.
+  apply kinds_generalize_disjoint.
+Qed.
+
+Lemma typing_let_disjoint : forall k EK0 e e0 s,
+  let K' := map (kind_subst s) k in
+  ok (e0 & e) -> is_subst s ->
+  ok K' -> env_incl (e0 & e) K' ->
+  disjoint (close_fvk K' EK0) (dom e) ->
+  dom e0 << close_fvk K' EK0 ->
+  disjoint (dom e) (EK0 \u dom (map (kind_subst s) e0)
+                    \u fv_in kind_fv (map (kind_subst s) e0)).
+Proof.
+  intros until K'; intros Ok Hs HK' Inc2 Dise Se0.
+  apply disjoint_comm.
+  repeat apply disjoint_union.
+  (* env_fv E *)
+  apply* disjoint_subset.
+  (* dom e0 *)
+  rewrite dom_map.
+  apply* ok_disjoint.
+  (* fv_in kind_fv (map (kind_subst s) e0) *)
+  refine (disjoint_subset (proj2 (fv_in_subset_inv _ _ _) _) Dise).
+  intros.
+  destruct (ok_concat_inv _ _ Ok).
+  use (in_ok_binds _ _ H (ok_map0 (kind_subst s) H0)).
+  apply* close_fvk_ok.
+    instantiate (1 := x).
+    use (binds_dom H2). rewrite dom_map in H3.
+    apply* Se0.
+  unfold K'.
+  rewrite <- (map_compose _ _ _ k (fun k => kind_subst_idem k Hs)).
+  destruct (binds_map_inv _ _ H2) as [b [Hb B]]. subst a.
+  apply binds_map.
+  apply* Inc2.
+Qed.
+
+Lemma typing_let_fresh : forall x l l0 k e e0 e1 e2 s fvE sK0,
+  let K' := map (kind_subst s) k in
+  let M := sch_generalize l (typ_subst s (typ_fvar x)) l0 in
+  split e2 = (l, l0) ->
+  ok (e0 & e) -> ok (e2 & e1) -> is_subst s ->
+  ok K' -> env_incl (e0 & e) K' -> env_incl (e2 & e1) e ->
+  disjoint (close_fvk K' (fvE \u sK0)) (dom e) ->
+  dom e0 << close_fvk K' (fvE \u sK0) ->
+  fresh
+    (fvE \u sch_fv M \u dom (map (kind_subst s) e0) \u
+     fv_in kind_fv (map (kind_subst s) e0)) (sch_arity M) l.
+Proof.
+  intros until M. intros R4 Ok Ok' Hs HK' Inc2 Inc4 Dise Se0.
+  unfold sch_arity; simpl length.
+  rewrite map_length.
+  rewrite <- (split_length _ R4).
+  use (split_combine e2). rewrite R4 in H.
+  apply* (ok_fresh l l0).
+    rewrite H. destruct* (ok_concat_inv _ _ Ok').
+  rewrite* <- (dom_combine l l0).
+  rewrite H.
+  use (env_incl_subset_dom Inc4).
+  rewrite dom_concat in H0.
+  assert (dom e2 << dom e).
+    intros v Hv. apply* (H0 v). auto with sets.
+  use (disjoint_subset H1
+          (typing_let_disjoint _ _ _ _ Ok Hs HK' Inc2 Dise Se0)).
+  assert (disjoint (sch_fv M) (dom e2)).
+    unfold M.
+    rewrite <- H.
+    rewrite* dom_combine.
+    apply sch_generalize_disjoint.
+  disjoint_solve.
+Qed.
+
+Lemma typing_let_fresh_2 : forall l1 l2 s k T fvE sK0 e e0 e1 e2,
+  let K' := map (kind_subst s) k in
+  let Ks := List.map (kind_map (typ_generalize l1)) l2 in
+  let M' := Sch T Ks in
+  is_subst s -> kenv_ok K' ->  ok (e0 & e) -> ok (e2 & e1) ->
+  env_incl (e0 & e) K' -> env_incl (e2 & e1) e ->
+  split e1 = (l1, l2) ->
+  disjoint (close_fvk K' (fvE \u sK0)) (dom e) ->
+  dom e0 << close_fvk K' (fvE \u sK0) ->
+  disjoint (close_fvk K' (typ_fv T)) (dom e1) ->
+  dom e2 << close_fvk K' (typ_fv T) ->
+  fresh
+    (fvE \u sch_fv M' \u dom (map (kind_subst s) e0 & e2) \u
+     fv_in kind_fv (map (kind_subst s) e0 & e2)) (sch_arity M') l1.
+Proof.
+  intros until M'.
+  intros Hs HK' Ok Ok' Inc2 Inc4 R5 Dise Se0 Dise1 Se2.
+  rewrite dom_concat; rewrite fv_in_concat.
+  unfold sch_arity; simpl length.
+  unfold Ks; rewrite map_length.
+  rewrite <- (split_length _ R5).
+  poses He1 (split_combine e1). rewrite R5 in He1.
+  apply* (ok_fresh l1 l2).
+    rewrite* He1. destruct* (ok_concat_inv _ _ Ok').
+  rewrite* <- (dom_combine l1 l2).
+  rewrite He1.
+  use (env_incl_subset_dom Inc4).
+  rewrite dom_concat in H.
+  assert (dom e1 << dom e).
+    intros v Hv. apply* (H v). auto with sets.
+  use (disjoint_subset H0
+         (typing_let_disjoint _ _ _ _ Ok Hs (proj1 HK') Inc2 Dise Se0)).
+  apply disjoint_comm.
+  repeat apply disjoint_union; try solve [disjoint_solve].
+  (* sch_fv M' *)
+  unfold sch_fv; simpl.
+  apply disjoint_union.
+    apply* disjoint_subset.
+  unfold Ks.
+  rewrite <- He1. rewrite* dom_combine.
+  apply kinds_generalize_disjoint.
+  (* e2 *)
+  refine (disjoint_subset (proj2 (fv_in_subset_inv _ _ _) _) Dise1).
+  intros.
+  destruct (ok_concat_inv _ _ Ok').
+  use (in_ok_binds _ _ H2 H3).
+  apply* close_fvk_ok.
+  apply Se2.
+  apply* binds_dom.
+Qed.
+
+Lemma sch_open_extra : forall Ks Xs T,
+  type T -> sch_open_vars (Sch T Ks) Xs = T.
+Proof.
+  unfold sch_open_vars, typ_open_vars; simpl; intros.
+  rewrite* <- typ_open_type.
+Qed.
+
+Lemma typing_let_incl : forall s k e e0 e1 e2,
+  let ss := map (kind_subst s) in
+  is_subst s ->
+  ok (e0 & e) -> ok (e2 & e1) ->
+  env_incl (ss k) (e0 & e) ->
+  env_incl (e0 & e) (ss k) ->
+  env_incl e (e2 & e1) ->
+  env_incl (e2 & e1) e ->
+  env_incl (ss k) (ss e0 & e2 & e1) /\ env_incl (ss e0 & e2 & e1) (ss k).
+Proof.
+  intros until ss; intros Hs Ok Ok' I1 I2 I3 I4.
+  rewrite concat_assoc.
+  set (e' := e2 & e1) in *.
+  split; intro; intros.
+    use (I1 _ _ H).
+    binds_cases H0.
+      apply binds_concat_fresh.
+        destruct (binds_map_inv _ _ H) as [k1 [Hk1 Bk1]].
+        subst.
+        use (binds_map (kind_subst s) B).
+        rewrite kind_subst_idem in H0; auto.
+      eapply notin_subset. apply (env_incl_subset_dom I4). auto.
+    use (I3 _ _ B0).
+  clearbody e'.
+  binds_cases H.
+    unfold ss.
+    rewrite* <- (map_compose (kind_subst s) (kind_subst s) (kind_subst s)).
+    apply (env_incl_map (kind_subst s) I2).
+    rewrite map_concat.
+    apply* binds_concat_fresh.
+    rewrite dom_map. eapply notin_subset.
+    apply (env_incl_subset_dom I3). auto.
+  auto.
+Qed.
+
+Lemma soundness_let : forall h t1 t2 K0 E T S0 S K,
+  (forall t K0 E T S0 K S, soundness_spec h t K0 E T S0 K S) ->
+  soundness_spec (Datatypes.S h) (trm_let t1 t2) K0 E T S0 K S.
+Proof.
+  intros until K; intros IHh  HI HS0 HTS0 HK0 Dis HE HSE HT; simpl in HI.
+  destruct (var_fresh (fvs S0 K0 E T)); simpl in HI.
+  case_rewrite (typinf K0 E t1 (typ_fvar x) S0 h) R1. destruct p.
+  fold (typ_subst s (typ_fvar x)) in HI.
+  set (K' := map (kind_subst s) k) in *.
+  set (T1 := typ_subst s (typ_fvar x)) in *.
+  case_rewrite (split_env (close_fvk K'
+    (env_fv (map (sch_subst s) E) \u vars_subst s (dom K0))) K') R2.
+  case_rewrite (split_env (close_fvk K' (typ_fv T1)) e) R3.
+  case_rewrite (split e2) R4.
+  destruct (var_fresh (dom E \u trm_fv t1 \u trm_fv t2)); simpl proj1_sig in HI.
+  set (M := sch_generalize l T1 l0) in *.
+  destruct* (IHh _ _ _ _ _ _ _ R1); clear R1.
+  destruct H0 as [HTs [Hs [Hk [Disk [WS' Typ']]]]].
+  assert (HT1: type T1) by (unfold T1; auto*).
+  assert (HK':kenv_ok K') by (unfold K'; apply* kenv_ok_map).
+  destruct* (split_env_ok _ R2) as [Ok [Dise [Se0 [Inc1 Inc2]]]].
+  destruct* (split_env_ok _ R3) as [Ok' [Dise' [Se2 [Inc3 Inc4]]]].
+    destruct* (ok_concat_inv _ _ Ok).
+  poses He2 (split_combine e2). rewrite R4 in He2.
+  assert (Oke0: ok e0) by destruct* (ok_concat_inv _ _ Ok).
+  assert (Oke2: ok e2) by destruct* (ok_concat_inv _ _ Ok').
+  assert (HM: scheme M).
+    unfold M.
+    apply* scheme_generalize.
+    apply* env_prop_list_forall.
+      rewrite He2.
+      intro; intros.
+      apply* (proj2 HK' x1).
+    rewrite* He2.
+  destruct* (IHh _ _ _ _ _ _ _ HI); clear IHh HI.
+          split*.
+          intro; destruct* HK'.
+        use (env_incl_subset_dom Inc2).
+        unfold K' in H0; rewrite dom_map in H0; rewrite dom_concat in H0.
+        intro v; destruct* (Disk v).
+        use (notin_subset H0 H1).
+      apply* ok_cons.
+    intro; intros.
+    unfold binds in H0; simpl in H0.
+    destruct (x1 == x0); subst.
+      inversions* H0.
+    apply (HSE _ _ H0).
+  intuition.
+      apply* extends_trans.
+    apply* well_subst_let_inf.
+  apply* (@typing_let (true,GcAny) (sch_subst S M)
+             (dom S \u dom K \u dom e0 \u mkset l)).
+    intros.
+    unfold M; simpl.
+    rewrite* <- kinds_subst_open_vars.
+    rewrite* <- sch_subst_open_vars.
+    fold M.
+    replace (List.map (kind_map (typ_generalize l)) l0) with (sch_kinds M)
+      by simpl*.
+    rewrite sch_arity_subst in H6.
+    rewrite <- (map_sch_subst_extend E H0).
+    apply* typing_typ_well_subst.
+        apply (well_subst_extend (sch_kinds M) Xs H2 H5).
+        rewrite* dom_map.
+      rewrite <- map_concat.
+      apply* kenv_ok_map.
+      apply* kenv_ok_sch_kinds.
+    assert (AryM: sch_arity M = length l).
+      unfold sch_arity; simpl.
+      rewrite map_length.
+      rewrite* (split_length _ R4).
+    apply* typing_rename_typ.
+        apply* (@typing_let_fresh x l l0 k e e0 e1 e2 s).
+      rewrite dom_map.
+      rewrite* <- AryM.
+    unfold M.
+    use (split_combine e2). rewrite R4 in H8.
+    assert (list_forall (All_kind_types type) l0).
+      apply* env_prop_list_forall.
+        rewrite H8. intro; intros. apply* (proj2 HK' x1).
+      rewrite* H8.
+    unfold sch_open_vars, typ_open_vars. simpl sch_type.
+    rewrite* typ_generalize_reopen.
+    unfold sch_generalize. simpl sch_kinds.
+    rewrite* kinds_generalize_reopen. rewrite H8. clear H9.
+    poses He1 (split_combine e1). case_rewrite (split e1) R5.
+    pose (Ks := List.map (kind_map (typ_generalize l1)) l2).
+    apply* (@typing_gc (true,GcAny) Ks). simpl*.
+    intros.
+    pose (M' := Sch T1 Ks).
+    rewrite* <- (@sch_open_extra Ks Xs0). fold M'.
+    replace Ks with (sch_kinds M') by simpl*.
+    apply* typing_rename_typ.
+        instantiate (1 := l1).
+        unfold M', Ks.
+        unfold K' in HK'.
+        apply* typing_let_fresh_2.
+      unfold Ks in H9. rewrite map_length in H9.
+      rewrite* (split_length _ R5).
+    assert (list_forall (All_kind_types type) l2).
+      apply* env_prop_list_forall.
+        rewrite He1. intro; intros. apply* (proj2 HK' x1).
+      rewrite* He1. destruct* (ok_concat_inv _ _ Ok').
+    simpl sch_kinds.
+    unfold Ks; rewrite* kinds_generalize_reopen. rewrite He1; clear H10.
+    unfold sch_open_vars, typ_open_vars.
+    simpl sch_type. rewrite* <- typ_open_type.
+    destruct* (typing_let_incl _ _ _ _ Hs Ok Ok' Inc1 Inc2 Inc3 Inc4).
+    unfold T1; apply* typing_kenv_incl.
+    split.
+      rewrite concat_assoc.
+      apply* disjoint_ok.
+      rewrite dom_map.
+      apply disjoint_comm.
+      eapply disjoint_subset. apply (env_incl_subset_dom Inc4).
+      apply disjoint_comm. apply* ok_disjoint.
+    intro; intros. apply* (proj2 (proj1 (typing_regular Typ')) x1).
+  intros.
+  instantiate (1 := dom E \u trm_fv t2 \u {{x0}}) in H6.
+  simpl gc_raise.
+  apply* (@typing_abs_rename x0).
+  rewrite* dom_map.
+Qed.
+
+Lemma soundness_app : forall h t1 t2 K0 E T S0 S K,
+  (forall t K0 E T S0 K S, soundness_spec h t K0 E T S0 K S) ->
+  soundness_spec (Datatypes.S h) (trm_app t1 t2) K0 E T S0 K S.
+Proof.
+  intros until K; intros IHh HI HS0 HTS0 HK0 Dis HE HSE HT; simpl in HI.
+  destruct (var_fresh (fvs S0 K0 E T)); simpl in HI.
+  case_rewrite (typinf K0 E t1 (typ_arrow (typ_fvar x) T) S0 h) R1.
+  destruct p as [K' S'].
+  destruct* (IHh _ _ _ _ _ _ _ R1); clear R1.
+  destruct* (IHh _ _ _ _ _ _ _ HI); clear IHh HI.
+  intuition.
+      apply* extends_trans.
+    apply* well_subst_compose.
+  remember (typ_fvar x) as T1.
+  apply* typing_app.
+  use (typing_typ_well_subst H0 H10 (kenv_ok_map H6 H0) H12).
+  rewrite (map_sch_subst_extend E H1) in H11.
+  rewrite H1 in H11.
+  apply H11.
+Qed.
+
+Theorem typinf_sound : forall h t K0 E T S0 K S,
+  soundness_spec h t K0 E T S0 K S.
 Proof.
   induction h; destruct t; intros;
     intros HI HS0 HTS0 HK0 Dis HE HSE HT; try discriminate.
   apply* (soundness_var h).
   apply* (@soundness_abs h).
+  apply* (@soundness_let h).
+  apply* (@soundness_app h).
+  apply* (soundness_cst h).
+Qed.
 
 End Mk2.
 End MkInfer.
